Seal inversions inside Intermediate interface
The price to pay to hide all the implementation details, at the moment,
is the addition of an auxiliary lemma that encapsulates the exposed
internals.

RSC_DC_MD.v
@@ -239,27 +239,11 @@ Module Type Intermediate_Sig.
     exists b3,
       program_behaves (CS.sem (program_link p c)) b3 /\ prefix m b3.
 
-  (* The top-level proof performs low-level manipulations on the now-abstract
-     definitions in a couple of places. These definitions must now become
-     opaque and exposed through the interface, and its operations given as
-     trivial inversion-type lemmas. We may want to think about removing these
-     noisy details through further abstraction.
-       [CH: We should indeed try to fix these bad abstraction leaks.] *)
-  Parameter prog_main : program -> option Procedure.id.
-
-  Parameter prog_procedures : program -> NMap (NMap code).
-
-  Hypothesis closed_program_inv : forall p,
-    closed_program p ->
-    closed_interface (prog_interface p) /\
-    exists mainP main_procs,
-      prog_main p = Some mainP /\
-      (prog_procedures p) Component.main = Some main_procs /\
-      mainP \in domm main_procs.
-
-  Hypothesis closed_interface_inv : forall p1 p2,
-    closed_interface (prog_interface (program_link p1 p2)) =
-    closed_interface (unionm (prog_interface p1) (prog_interface p2)).
+  Hypothesis compose_mergeable_interfaces :
+    forall p c,
+      linkable (prog_interface p) (prog_interface c) ->
+      closed_program (program_link p c) ->
+      mergeable_interfaces (prog_interface p) (prog_interface c).
 End Intermediate_Sig.
 
 Module Intermediate_Instance <: Intermediate_Sig.
@@ -315,36 +299,8 @@ Module Intermediate_Instance <: Intermediate_Sig.
   Definition composition_prefix :=
     @Intermediate.Composition.composition_prefix.
 
-  (* The following additions are required by the top-level proof to perform
-     some basic manipulations that the standard Coq tactics cannot handle once
-     we hide Intermediate behind an interface. Inversion lemmas to replace
-     simple destructs and rewrites are, of course, trivial: these do not need
-     to be added to our instance's Intermediate.
-       [CH: We should indeed try to fix these bad abstraction leaks.] *)
-
-  Definition prog_main :=
-    @Intermediate.prog_main.
-
-  Definition prog_procedures :=
-    @Intermediate.prog_procedures.
-
-  Lemma closed_program_inv : forall p,
-    closed_program p ->
-    closed_interface (prog_interface p) /\
-    exists mainP main_procs,
-      prog_main p = Some mainP /\
-      (prog_procedures p) Component.main = Some main_procs /\
-      mainP \in domm main_procs.
-  Proof.
-    by intros p [Hclosed Hmain].
-  Qed.
-
-  Lemma closed_interface_inv : forall p1 p2,
-    closed_interface (prog_interface (program_link p1 p2)) =
-    closed_interface (unionm (prog_interface p1) (prog_interface p2)).
-  Proof.
-    easy.
-  Qed.
+  Definition compose_mergeable_interfaces :=
+    @Intermediate.compose_mergeable_interfaces.
 End Intermediate_Instance.
 
 Module Type S2I_Sig (Source : Source_Sig) (Intermediate : Intermediate_Sig).
@@ -738,6 +694,8 @@ Section RSC_DC_MD_Section.
       exact: Source.linking_well_formedness well_formed_P' well_formed_Cs linkability_pcomp_Ct.
     have HP'_Cs_compiled_beh : program_behaves (Intermediate.CS.sem P'_Cs_compiled) beh.
       have sim := Compiler.I_simulates_S HP'Cs_closed well_formed_P'Cs HP'_Cs_compiles.
+      pose proof forward_simulation_same_safe_prefix.
+      Print does_prefix.
       exact: (forward_simulation_same_safe_behavior sim).
 
     (* intermediate decomposition (for Cs_compiled) *)
@@ -802,17 +760,9 @@ Section RSC_DC_MD_Section.
     assert (mergeable_interfaces (Intermediate.prog_interface p_compiled)
                                  (Intermediate.prog_interface Cs_compiled))
       as Hmergeable_ifaces.
-    {
-      split.
-      - assumption.
-      - apply Intermediate.closed_program_inv in HpCs_compiled_closed.
-        destruct HpCs_compiled_closed
-          as [HpCs_compiled_closed_interface HpCs_compiled_closed_main].
-        erewrite <- Intermediate.closed_interface_inv.
-        assumption.
-    }
+      by apply Intermediate.compose_mergeable_interfaces.
 
-    destruct HP_decomp as [b1 [Hbehvesb1 Hprefixb1]]. 
+    destruct HP_decomp as [b1 [Hbehvesb1 Hprefixb1]].
 
     pose proof Intermediate.composition_prefix
          well_formed_p_compiled well_formed_Cs_compiled
